Define and prove lemmas about high-level store in Vale sems

src/test/interop/Low_Sem.fst
@@ -17,8 +17,19 @@ let buffer_read (b:buffer64) (i:nat{i < B.length b}) (mem:HS.mem) : GTot nat64 =
   let contents = B.as_seq mem b in
   UInt64.v (Seq.index contents i)
 
-let buffer_write (b:buffer64) (i:nat{i < B.length b}) (v:nat64) (mem:HS.mem) : GTot HS.mem =
-  admit()
+val buffer_write: b:buffer64 -> (n:nat{n < B.length b}) -> v:nat64 -> (h0:HS.mem{B.live h0 b}) -> GTot
+ (h1:HS.mem)
+ 
+let buffer_write b n v h0 =
+ let s0 = B.sel h0 b in
+// assume (B.idx b + B.length b <= B.max_length b);
+// assume (B.max_length b == Seq.Base.length s0);
+// assume (0 <= B.idx b + n /\ B.idx b + n < B.max_length b);
+ let s = Seq.upd s0 (B.idx b + n) (UInt64.uint_to_t v) in
+// assume (HS.live_region h0 (B.frameOf b));
+ let h1 = HS.upd h0 (B.content b) s in
+// lemma_aux #a b n z h0;
+ h1
 
 noeq type low_state_p = {
   s:M.state;
@@ -27,11 +38,12 @@ noeq type low_state_p = {
   mem: HS.mem;
 }
 
-let valid_state s =
-  list_disjoint_or_eq s.ptrs /\
+type low_state = (s:low_state_p{list_disjoint_or_eq s.ptrs /\ list_live s.mem s.ptrs})
+
+let valid_state (s:low_state) =
   s.s.M.mem == down_mem64 s.mem s.addrs s.ptrs
 
-type low_state = (s:low_state_p{valid_state s})
+// type low_state = (s:low_state_p{valid_state s})
 
 val valid_mem: ptr:int 
   -> s:low_state
@@ -43,6 +55,7 @@ val store_mem: ptr:int
   -> v:nat64 
   -> s:low_state
   -> GTot low_state
+
 
 val addr_in_ptr: (addr:int) -> (ptr:buffer64) -> (addrs:addr_map) ->
   GTot (b:bool{ not b <==> (forall i. 0 <= i /\ i < B.length ptr ==> 
@@ -60,6 +73,13 @@ let addr_in_ptr (addr:int) (ptr:buffer64) (addrs:addr_map) =
     else aux (i+1)
   in aux 0
 
+let rec get_addr_in_ptr (n base addr:nat) (i:nat{exists j. i <= j /\ j < n /\ base + 8 `op_Multiply` j == addr}) : 
+    GTot (j:nat{base + 8 `op_Multiply` j == addr})
+    (decreases %[n-i]) =
+    if base + 8 `op_Multiply` i = addr then i
+    else if i >= n then i
+    else get_addr_in_ptr n base addr (i+1)
+
 
 let rec valid_mem_aux addr ps (addrs:addr_map) : GTot (b:bool{
   (not b) <==> (forall (x:buffer64). (List.memP x ps ==> not (addr_in_ptr addr x addrs) ))}) 
@@ -71,12 +91,26 @@ let valid_mem addr s =
   // Iterate over the list of buffers existing in this state
   valid_mem_aux addr s.ptrs s.addrs
 
-
 let load_mem ptr s = M.get_heap_value ptr s.s
+
+let rec store_mem_aux addr ps (v:nat64) (addrs:addr_map) (h0:HS.mem{list_live h0 ps}) : 
+  GTot (h1:HS.mem{forall (b:buffer64). B.live h0 b <==> B.live h1 b }) =
+  match ps with
+  | [] -> h0
+  | a::q ->
+    let base = buffer_addr a addrs in
+    let n = B.length a in
+    if addr_in_ptr addr a addrs then
+    begin
+//      buffer_write a 0 v h0
+      buffer_write a (get_addr_in_ptr n base addr 0) v h0
+    end
+    else store_mem_aux addr q v addrs h0
 
 let store_mem ptr v s =
   let s' = M.update_mem ptr v s.s in
-  admit()
+  let h1 = store_mem_aux ptr s.ptrs v s.addrs s.mem in
+  {s with s = s'; mem = h1}
 
 let rec valid_mem_aux_lemma addr ps addrs (x:buffer64) : Lemma (
    List.memP x ps /\ addr_in_ptr addr x addrs ==>
@@ -89,7 +123,7 @@ let rec valid_mem_aux_lemma addr ps addrs (x:buffer64) : Lemma (
 val lemma_valid_mem: b:buffer64
   -> i:nat 
   -> s:low_state
-  -> Lemma (requires i < B.length b /\ List.memP b s.ptrs)
+  -> Lemma (requires i < B.length b /\ List.memP b s.ptrs /\ valid_state s)
      (ensures valid_mem 
        (buffer_addr b s.addrs + 8 `op_Multiply` i)
        s)
@@ -102,7 +136,7 @@ let lemma_valid_mem b i s =
 val lemma_load_mem: b:buffer64
   -> i:nat
   -> s:low_state
-  -> Lemma (requires i < B.length b /\ List.memP b s.ptrs)
+  -> Lemma (requires i < B.length b /\ List.memP b s.ptrs /\ valid_state s)
      (ensures load_mem (buffer_addr b s.addrs + 8 `op_Multiply` i) s == buffer_read b i s.mem)
 
 let lemma_load_mem b i s = ()
@@ -111,8 +145,9 @@ val lemma_store_mem: b:buffer64
   -> i:nat 
   -> v:nat64
   -> s:low_state
-  -> Lemma (requires i < B.length b /\ List.memP b s.ptrs)
-     (ensures (store_mem (buffer_addr b s.addrs + 8 `op_Multiply` i) v s).mem == buffer_write b i v s.mem)
+  -> Lemma (requires i < B.length b /\ List.memP b s.ptrs /\ valid_state s)
+     (ensures (let s' = store_mem (buffer_addr b s.addrs + 8 `op_Multiply` i) v s in
+       s'.mem == buffer_write b i v s.mem))
 
 val lemma_store_load_mem: i:int 
   -> v:nat64
@@ -131,3 +166,102 @@ val lemma_valid_store_mem: i:int
   -> s:low_state
   -> Lemma (let s' = store_mem i v s in
      forall j. valid_mem j s <==> valid_mem j s')
+
+val lemma_valid_state_store_mem: i:int 
+  -> v:nat64
+  -> s:low_state
+  -> Lemma (requires (valid_state s /\ valid_mem i s))
+    (ensures valid_state (store_mem i v s))
+
+#set-options "--z3rlimit 20"
+
+let valid_disjoint i i' s : Lemma 
+  (valid_mem i s /\ valid_mem i' s /\ i' <> i ==> i' + 8 <= i \/ i + 8 <= i') =
+  let rec aux addrs (ps:list buffer64{list_disjoint_or_eq ps}) : Lemma 
+  (requires (i <> i' /\ valid_mem_aux i ps addrs /\ valid_mem_aux i' ps addrs))
+  (ensures (i' + 8 <= i \/ i + 8 <= i')) =
+  match ps with
+  | [] -> ()
+  | a::q -> 
+    if (addr_in_ptr i a addrs) then
+      if (addr_in_ptr i' a addrs) then ()
+      else
+      let rec aux2 (ps2:list buffer64{list_disjoint_or_eq (a::ps2)}) : Lemma
+      (requires valid_mem_aux i' ps2 addrs)
+      (ensures (i' + 8 <= i \/ i + 8 <= i')) =
+      match ps2 with
+    	| [] -> ()
+    	| b::r -> 
+	  if (addr_in_ptr i' b addrs) then begin
+	    assert (disjoint_or_eq a b);
+	    ()
+	  end
+	  else aux2 r
+      in aux2 q
+    else begin 
+      if (addr_in_ptr i' a addrs) then begin
+      let rec aux2 (ps2:list buffer64{list_disjoint_or_eq (a::ps2)}) : Lemma
+	(requires valid_mem_aux i ps2 addrs)
+	(ensures (i' + 8 <= i \/ i + 8 <= i')) =
+	match ps2 with
+    	  | [] -> ()
+    	  | b::r -> 
+	    if (addr_in_ptr i b addrs) then begin
+	      assert (disjoint_or_eq a b);
+	      ()
+	    end
+	    else aux2 r
+	in aux2 q	
+      end
+      else aux addrs q
+    end
+  in
+  Classical.move_requires (aux s.addrs) s.ptrs
+
+let lemma_store_mem b i v s =
+  let addr = buffer_addr b s.addrs + 8 `op_Multiply` i in
+  let s' = store_mem addr v s in
+  let rec aux (ps:list buffer64{list_disjoint_or_eq ps}) (h0:HS.mem{list_live h0 ps}) : 
+    Lemma (requires (valid_state s /\ List.memP b ps /\ i < B.length b) )
+    (ensures (store_mem_aux addr ps v s.addrs h0 == buffer_write b i v h0)) = 
+  match ps with
+    | [] -> ()
+    | a::q ->
+      if addr_in_ptr addr a s.addrs then begin
+	assert (disjoint_or_eq a b);
+	()
+      end
+      else begin
+	assert (b =!= a);
+	aux q h0
+      end
+  in aux s.ptrs s.mem
+
+let lemma_store_load_mem i v s = ()
+
+let lemma_frame_store_mem i v s =
+  let s' = store_mem i v s in
+  let rec aux i' : Lemma (i' <> i /\ valid_mem i s /\ valid_mem i' s ==>
+    load_mem i' s = load_mem i' s') =
+    valid_disjoint i i' s;
+    M.frame_update_heap i v s.s.M.mem;
+    ()
+  in Classical.forall_intro aux 
+
+let lemma_valid_store_mem i v s = ()
+
+let store_buffer_down_mem (b:buffer64) (i:nat{i < B.length b}) (v:nat64)
+  (ps: list buffer64{list_disjoint_or_eq ps /\ List.memP b ps}) (h0:HS.mem{list_live h0 ps}) (addrs:addr_map) :
+  Lemma (
+    let mem1 = down_mem64 h0 addrs ps in
+    let h1 = buffer_write b i v h0 in
+    let mem2 = down_mem64 h1 addrs ps in
+    let base = buffer_addr b addrs in
+    forall j. j < base + 8 `op_Multiply` i \/ j >= base + 8 `op_Multiply` (i+1) ==>
+      mem1.[j] == mem2.[j]) = admit()
+
+let lemma_valid_state_store_mem i v s =
+  let s' = store_mem i v s in
+  assert (s.s.M.mem == down_mem64 s.mem s.addrs s.ptrs);
+  assert (s'.s == M.update_mem i v s.s);
+  assume (s'.s.M.mem == down_mem64 s'.mem s.addrs s.ptrs)
